define quarterround inverse theorems

src/salsa20/quarterround.lean
@@ -32,9 +32,51 @@ def quarterround (y : vector (bitvec word_len) 4) : vector (bitvec word_len) 4 :
 lemma quarterround_zero : 
   (quarterround (subtype.mk [0, 0, 0, 0] (by refl))).to_list = [0, 0, 0, 0] := rfl
 
--- TODO: The whole quarterround function is invertible
+-- The whole quarterround function is invertible because individual vector components are invertible.
+-- From z = [z₀, z₁, z₂, z₃] we can get back to [y₀, y₁, y₂, y₃]
+
+-- The interesting thing is that it seems we don't need to apply the inverses of rotl and zmod
+-- addition, instead to get yₓ we just replace zₓ in the original formula and compute. 
+
+-- y₀ = z₀ ⊕ ((z₃ + z₂) <<< 18)
+def y₀ (z : vector (bitvec word_len) 4) : bitvec word_len := 
+  bitvec.xor (z.nth 0) (rotl (nat_as_bitvec (mod_as_nat (add_bitvecs_as_mod (z.nth 3) (z.nth 2)))) 18) 
+
+-- y₃ = z₃ ⊕ ((z₂ + z₁) <<< 13)
+def y₃ (z : vector (bitvec word_len) 4) : bitvec word_len := 
+  bitvec.xor (z.nth 3) (rotl (nat_as_bitvec (mod_as_nat (add_bitvecs_as_mod (z.nth 2) (z.nth 1)))) 13) 
+
+-- y₂ = z₂ ⊕ ((z₁ + y₀) <<< 9)
+def y₂ (z : vector (bitvec word_len) 4) : bitvec word_len := 
+  bitvec.xor (z.nth 2) (rotl (nat_as_bitvec (mod_as_nat (add_bitvecs_as_mod (z.nth 1) (y₀ z)))) 9) 
+
+-- y₁ = z₁ ⊕ ((y₀ + y₃) <<< 7)
+def y₁ (z : vector (bitvec word_len) 4) : bitvec word_len := 
+  bitvec.xor (z.nth 1) (rotl (nat_as_bitvec (mod_as_nat (add_bitvecs_as_mod (y₀ z) (y₃ z)))) 7) 
+
+-- The inverse of the quarterround function puts together the above definitions for the 
+-- components of y.
 def quarterround_inv (z : vector (bitvec word_len) 4) : vector (bitvec word_len) 4 :=
-  do 
-    sorry
+  subtype.mk [
+    y₀ z,
+    y₁ z,
+    y₂ z,
+    y₃ z
+  ] (by refl)
+
+-- double quarterround is not the inverse
+lemma double_quarterround_not_inverse (y : vector (bitvec word_len) 4) : quarterround (quarterround y) ≠ y :=
+begin
+  sorry,
+end
+
+-- quarterround_inv is the inverse
+lemma quarterround_inv_is_inverse (y : vector (bitvec word_len) 4) : y = quarterround_inv (quarterround y) :=
+begin
+  unfold quarterround_inv,
+  unfold quarterround,
+  sorry,
+end
+
 
 end quarterround
